new-stuff/binary-tree-search.dfy
@@ -1,0 +1,20 @@
+include "binary-tree.dfy"
+
+method FindInBinaryTree(t:Tree, needle:int) returns (b:bool)
+    requires IsSortedTree(t)
+    ensures b <==> needle in I(t)
+{
+    if (t.Nil?) {
+        return false;
+    } else {
+        if (needle == t.value) {
+            return true;
+        } else if (needle < t.value) {
+            var leftRet := FindInBinaryTree(t.left, needle);
+            return leftRet;
+        } else {
+            var rightRet := FindInBinaryTree(t.right, needle);
+            return rightRet;
+        }
+    }
+}
